I2MP/Examples/Increment.v
@@ -11,7 +11,7 @@ Extraction "/tmp/run_tagged_compiled_increment.ml" to_run_tr.
 
 Require Import Merged Int32 I2MP.Examples.Helper.
 
-Definition to_run_mr := @Merged.compile_and_run_from_source_merged_ex concrete_int_32_mt increment fuel.
+Definition to_run_mr := @Merged.compile_and_run_from_source_merged_ex concrete_int_32_mt concrete_int_32_ops increment fuel.
 (*
 Definition to_run_mr := @I2MP.Examples.Helper.compile_and_run_and_show_from_source_merged concrete_int_32_mt increment fuel. *)
 Set Warnings "-extraction-reserved-identifier".
