MicroPolicies/Recomposition.v
@@ -1,0 +1,60 @@
+Require Import Common.Definitions.
+
+From CoqUtils Require Import hseq word.
+From extructures Require Import fmap.
+From mathcomp Require Import ssreflect ssrfun ssrbool eqtype ssrnat seq.
+Require Import Symbolic Types.
+Export Symbolic.
+Require MicroPolicies.Merged.
+Require Import MicroPolicies.Utils MicroPolicies.LRC Intermediate.Machine.
+Require Import  MicroPolicies.Int32.
+Require Import CompCert.Events.
+
+
+Require Import Source.Language S2I.Compiler.
+Require Export Extraction.Definitions.
+
+
+Set Implicit Arguments.
+Unset Strict Implicit.
+Unset Printing Implicit Defensive.
+Import DoNotation.
+
+
+Context {mt : machine_types} {ops : machine_ops mt} {sregs : syscall_regs mt}.
+
+Definition step_eval_mp := (@Exec.stepf mt ops sym_lrc Merged.table_lrc).
+Definition step_eval_me := (@Exec.stepf mt ops Merged.sym_lrc_merged Merged.table).
+Definition step_mp := (@Symbolic.step mt ops sym_lrc Merged.table_lrc).
+Definition step_me := (@Symbolic.step mt ops Merged.sym_lrc_merged Merged.table).
+
+Notation state := (state sym_lrc).
+
+Definition id (s:state) : @Symbolic.state mt Merged.sym_lrc_merged :=
+  Symbolic.State Merged.sym_lrc_merged (Symbolic.mem s) (Symbolic.regs s) (Symbolic.pc s) (Symbolic.internal s) (Symbolic.comp_num s).
+
+Inductive trace_prod : state -> state -> trace -> Type :=
+| trace_refl : forall s, trace_prod s s nil
+| trace_step_nil : forall s1 s2 s3 t,
+    (step_mp s2 s3 None)
+     -> trace_prod s1 s2 t
+     -> trace_prod s1 s3 t
+| trace_step_ev : forall s1 s2 s3 t ev,
+    (step_mp s2 s3 (Some ev))
+     -> trace_prod s1 s2 t
+     -> trace_prod s1 s3 (ev :: t).
+
+Definition undefined_behavior s : Prop :=
+  exists out, (step_eval_mp s = Some out) /\ (step_eval_me (id s) = None).
+
+Definition undefined_behavior_in_P c s : Prop :=
+  exists v,
+  (undefined_behavior s) /\ ((mem s) (vala (pc s)) = Some v ) /\ ((color (taga v)) = c).
+
+Fixpoint trace_prod_satisfy {s s' t} (tp : trace_prod s s' t) P : Prop :=
+  match tp with
+  | trace_refl s => P s
+  | trace_step_nil _ _ s3 _ _ tp'
+  | trace_step_ev  _ _ s3 _ _ _ tp' => (P s3) /\ (trace_prod_satisfy tp' P)
+  end.
+                                                          
